& \overrightarrow {a} =
\begin{align}
    \begin{bmatrix}
        6 \\
        -2 \\
    \end{bmatrix}
\end{align},
\overrightarrow {b} =
\begin{align}
    \begin{bmatrix}
        -4 \\
        4 \\
    \end{bmatrix}
\end{align} \\
\\
& \overrightarrow {a}+\overrightarrow {b} \\
& = \begin{align}
    \begin{bmatrix}
        6 \\
        -2 \\
    \end{bmatrix}
\end{align} +
\begin{align}
    \begin{bmatrix}
        -4 \\
        4 \\
    \end{bmatrix}
\end{align} \\
& = â€‹\begin{align}
    \begin{bmatrix}
        6+(-4) \\
        -2+4 \\
    \end{bmatrix}
\end{align} \\
& = \begin{align}
    \begin{bmatrix}
        2 \\
        -2 \\
    \end{bmatrix}
\end{align}